\documentclass[a4paper,10pt]{article}
\usepackage[utf8]{inputenc}
\usepackage{amsmath}

%opening
\title{Preuve}
\author{}

\begin{document}

\maketitle

\begin{abstract}

\end{abstract}

\section{}
\[[\nabla_{x} \frac{1}{2}||Ax - b||^{2}_{2}]_{j} = [\nabla_{x} \frac{1}{2}(Ax - b).(Ax - b)]_{j}\]
\[[\nabla_{x} \frac{1}{2}||Ax - b||^{2}_{2}]_{j} = [\nabla_{x} \frac{1}{2}(\sum^{n}_{i = 1} (\sum^{p}_{k = 1} A_{i, k}x_{k})^{2} - 2b_{i}(\sum^{p}_{k = 1} A_{i, k}x_{k}) + b_{i}^{2})]_{j}\]
\[[\nabla_{x} \frac{1}{2}||Ax - b||^{2}_{2}]_{j} = \frac{\partial\frac{1}{2}(\sum^{n}_{i = 1} (\sum^{p}_{k = 1} A_{i, k}x_{k})^{2} - 2b_{i}(\sum^{p}_{k = 1} A_{i, k}x_{k}) + b_{i}^{2})}{\partial x_{j}}\]
\[[\nabla_{x} \frac{1}{2}||Ax - b||^{2}_{2}]_{j} = \frac{1}{2}(\sum^{n}_{i = 1} 2(\sum^{p}_{k = 1} A_{i, k}x_{k})A_{i, j} - 2b_{i} A_{i, j}) \]
\[[\nabla_{x} \frac{1}{2}||Ax - b||^{2}_{2}]_{j} = (\sum^{n}_{i = 1} (\sum^{p}_{k = 1} A_{i, k}x_{k})A_{i, j} - b_{i} A_{i, j}) \]
\[[\nabla_{x} \frac{1}{2}||Ax - b||^{2}_{2}]_{j} = (\sum^{n}_{i = 1} A_{i, j}(\sum^{p}_{k = 1} A_{i, k}x_{k}) - b_{i} ) \]
\[[\nabla_{x} \frac{1}{2}||Ax - b||^{2}_{2}]_{j} = \sum^{n}_{i = 1} A^{T}_{j, i}[Ax - b]_{i}\]
\[[\nabla_{x} \frac{1}{2}||Ax - b||^{2}_{2}]_{j} = [A^{T}(Ax - b)]_{j}\]
\end{document}
